update the sp typeclass

theories/contract.v
@@ -11,7 +11,7 @@
     semantics (according to a certain definition of “correct”). *)
 
 From mathcomp Require Import ssreflect.
-From FreerDPS Require Import effect freer.
+From FreerDPS Require Import effect freer mathcomp_extra.
 From HB Require Import structures.
 #[local]
 Open Scope signature_scope.
@@ -252,9 +252,10 @@ Infix "-*-" := contractprod (at level 20) : contract_scope .
 
 (** We also introduce a second composition operator which shares the
     witness state among its two operands. *)
-
-Definition sharedcontractprod {Fx F E : effect}
-    `{StrictProvide2 Fx F E}
+Section s.
+Context {Fx : effect}.
+Definition sharedcontractprod {F E : effect}
+    `{F -< Fx, E -< Fx} `{F ;; E -<< Fx}
     {Ω : Type} (ci : contract F Ω) (cj : contract E Ω)
   : contract Fx Ω :=
   {|
@@ -274,8 +275,8 @@ Definition sharedcontractprod {Fx F E : effect}
       gen_callee_obligation ci ω e x /\ gen_callee_obligation cj ω e x
   |}.
 
+End s.
 Infix "-^-" := sharedcontractprod (at level 20, right associativity) : contract_scope.
-
 (** * Contract By Example *)
 
 (** Finally, and as an example, we define a contract for the effect
@@ -342,12 +343,14 @@ Definition store_specs (s : Type) : contract (STORE s) s :=
 
 
 Section contract_helpers.
-Context {Fx F : effect} {Hfxf : F -< Fx} {W X Y : Type}
+Context {Fx F : effect} `{F -< Fx} {W X Y : Type}
     (c : contract F W) (w w' : W) (op : F X) (op' : F Y)
     (x : X) (concl : Prop).
 
+Local Notation inj := (inj (Fx:=Fx)).
+
 Lemma provided_callerP :
-  gen_caller_obligation (H := Hfxf.(may_prov)) c w (inj op)
+  gen_caller_obligation c w (inj op)
   <-> caller_obligation c w op.
 Proof.
 by rewrite /gen_caller_obligation !injK_Some.
@@ -356,9 +359,9 @@ Qed.
 Lemma provided_bind_caller :
   (callee_obligation c w op x ->
     caller_obligation c (witness_update c w op x) op') ->
-  gen_callee_obligation (H := Hfxf.(may_prov)) c w (inj op) x ->
-  gen_caller_obligation (H := Hfxf.(may_prov)) c
-    (gen_witness_update (H := Hfxf.(may_prov)) c w (inj op) x)
+  gen_callee_obligation c w (inj op) x ->
+  gen_caller_obligation c
+    (gen_witness_update c w (inj op) x)
     (inj op').
 Proof.
 rewrite /gen_witness_update /gen_callee_obligation.
@@ -367,65 +370,31 @@ Qed.
 
 
 Lemma provided_calleeP :
-  (w' = gen_witness_update (H := Hfxf.(may_prov)) c w (inj op) x /\ gen_callee_obligation (H := Hfxf.(may_prov)) c w (inj op) x )
+  (w' = gen_witness_update c w (inj op) x
+  /\ gen_callee_obligation c w (inj op) x )
   <-> (w' = witness_update c w op x /\ callee_obligation c w op x) .
 Proof.
 by split; rewrite /gen_callee_obligation /gen_witness_update !injK_Some.
 Qed.
 
-(* Lemma provided_callee :
-  (callee_obligation c w op x ->
-    w' = witness_update c w op x) <->
-  (gen_callee_obligation (H := Hfxf.(may_prov)) c w (inj op) x ->
-  w' = gen_witness_update (H := Hfxf.(may_prov)) c w (inj op) x).
-Proof.
-by split; rewrite /gen_callee_obligation /gen_witness_update !injK_Some.
-Qed.
-
-Lemma provided_callee_run :
-  (callee_obligation c w op x ->
-    w' = witness_update c w op x -> concl) ->
-  gen_callee_obligation (H := Hfxf.(may_prov)) c w (inj op) x ->
-  w' = gen_witness_update (H := Hfxf.(may_prov)) c w (inj op) x ->
-  concl.
-Proof.
-by rewrite /gen_callee_obligation /gen_witness_update !injK_Some.
-Qed.
-
-Lemma provided_callee_bind_run :
-  (callee_obligation c w op x ->
-    (exists y : Y,
-      w' = witness_update c (witness_update c w op x) op' y /\
-      callee_obligation c (witness_update c w op x) op' y) ->
-    concl) ->
-  gen_callee_obligation (H := Hfxf.(may_prov)) c w (inj op) x ->
-  (exists y : Y,
-    w' = gen_witness_update (H := Hfxf.(may_prov)) c
-      (gen_witness_update (H := Hfxf.(may_prov)) c w (inj op) x)
-      (inj op') y /\
-    gen_callee_obligation (H := Hfxf.(may_prov)) c
-      (gen_witness_update (H := Hfxf.(may_prov)) c w (inj op) x)
-      (inj op') y) ->
-  concl.
-Proof.
-by rewrite /gen_callee_obligation /gen_witness_update !injK_Some.
-Qed. *)
 End contract_helpers.
 
 Section contract_distinguish_helpers.
-Context {Fx F G : effect} {Hfxf : F -<? Fx} {Hfxg : G -< Fx}
-    {Hdist : @Distinguish Fx G F Hfxg Hfxf}
+Context {Fx F G : effect} `{F -<? Fx} `{G -< Fx}
+    `{Distinguish Fx G F}
     {W X : Type} (c : contract F W) (w w' : W) (op : G X) (x : X).
 
+Local Notation inj := (inj (Fx:=Fx)).
+
 Lemma distinguished_caller :
-  gen_caller_obligation (H := Hfxf) c w (inj op).
+  gen_caller_obligation c w (inj op).
 Proof.
 by rewrite /gen_caller_obligation injK_None.
 Qed.
 
 Lemma distinguished_callee :
-  (w' = gen_witness_update (H := Hfxf) c w (inj op) x /\
-    gen_callee_obligation (H := Hfxf) c w (inj op) x) <->
+  (w' = gen_witness_update c w (inj op) x /\
+    gen_callee_obligation c w (inj op) x) <->
   w' = w.
 Proof.
 rewrite /gen_witness_update /gen_callee_obligation injK_None.
@@ -435,17 +404,20 @@ End contract_distinguish_helpers.
 
 
 Section shared_contract_helpers.
-Context {Fx F G : effect} `{StrictProvide2 Fx F G}
+Context {Fx F G : effect}.
+Context `{S: F;; G -<< Fx}
     {W X : Type} (ci : contract F W) (cj : contract G W)
     (w w' : W) (x : X).
 
+Local Notation inj := (inj (Fx:=Fx)).
+
 Lemma shared_left_callerP (op : F X) :
-  gen_caller_obligation (Fx := Fx)
-    (sharedcontractprod (Fx := Fx) ci cj) w (inj (Fx := Fx) op)
+  gen_caller_obligation
+    (ci -^- cj) w (inj op)
   <-> caller_obligation ci w op.
 Proof.
 split.
-- by case=> + _; rewrite provided_callerP.
+- Set Printing Implicit. by case=> + _; rewrite provided_callerP.
 - move=> caller; split.
   + rewrite provided_callerP; exact: caller.
   + by rewrite /gen_caller_obligation (@injK_None Fx F G).
@@ -453,7 +425,7 @@ Qed.
 
 Lemma shared_right_callerP (op : G X) :
   gen_caller_obligation (Fx := Fx)
-    (sharedcontractprod (Fx := Fx) ci cj) w (inj (Fx := Fx) op)
+    (ci -^- cj) w (inj op)
   <-> caller_obligation cj w op.
 Proof.
 split.
@@ -465,11 +437,11 @@ Qed.
 
 Lemma shared_left_calleeP (op : F X) :
   (w' = gen_witness_update (Fx := Fx)
-      (sharedcontractprod (Fx := Fx) ci cj) w
-      (inj (Fx := Fx) op) x /\
+      (ci -^- cj) w
+      (inj op) x /\
     gen_callee_obligation (Fx := Fx)
-      (sharedcontractprod (Fx := Fx) ci cj) w
-      (inj (Fx := Fx) op) x) <->
+      (ci -^- cj) w
+      (inj op) x) <->
   w' = witness_update ci w op x /\ callee_obligation ci w op x.
 Proof.
 rewrite /gen_witness_update /gen_callee_obligation /=.
@@ -480,11 +452,11 @@ Qed.
 
 Lemma shared_right_calleeP (op : G X) :
   (w' = gen_witness_update (Fx := Fx)
-      (sharedcontractprod (Fx := Fx) ci cj) w
-      (inj (Fx := Fx) op) x /\
+      (ci -^- cj) w
+      (inj op) x /\
     gen_callee_obligation (Fx := Fx)
-      (sharedcontractprod (Fx := Fx) ci cj) w
-      (inj (Fx := Fx) op) x) <->
+      (ci -^- cj) w
+      (inj op) x) <->
   w' = witness_update cj w op x /\ callee_obligation cj w op x.
 Proof.
 rewrite /gen_witness_update /gen_callee_obligation /=.
@@ -493,3 +465,70 @@ rewrite (@injK_None Fx G F) (@injK_Some Fx G).
 by tauto.
 Qed.
 End shared_contract_helpers.
+
+
+(******************************************************************************)
+(******************************************************************************)
+(******************************************************************************)
+
+Section shared_contract_inj_helpers.
+Context {H Fx F G : effect} `{F;; G-<<Fx, Fx -< H}
+    {W X : Type} (ci : contract F W) (cj : contract G W)
+    (w w' : W) (x : X).
+
+Local Notation inj := (inj (Fx:=Fx)).
+
+Lemma shared_left_caller_injP (op : F X) :
+  gen_caller_obligation
+    (sharedcontractprod (Fx:=Fx) ci cj) w (effect.injT H Fx F _ op)
+  <-> caller_obligation ci w op.
+Proof.
+split; rewrite provided_callerP /= provided_callerP.
+- by case=> + _.
+- move=> caller; split.
+  + exact: caller.
+  + by rewrite /gen_caller_obligation (@injK_None Fx F G).
+Qed.
+
+Lemma shared_right_caller_injP (op : G X) :
+  gen_caller_obligation
+    (ci -^- cj) w (effect.injT H Fx G _ op)
+  <-> caller_obligation cj w op.
+Proof.
+split; rewrite provided_callerP /= provided_callerP.
+- by case=> _.
+- move=> caller; split.
+  + by rewrite /gen_caller_obligation (@injK_None Fx G F).
+  + exact: caller.
+Qed.
+
+Lemma shared_left_callee_injP (op : F X) :
+  (w' = gen_witness_update
+      (ci -^- cj) w
+      (effect.injT H Fx F _ op) x /\
+    gen_callee_obligation
+      (ci -^- cj) w
+      (effect.injT H Fx F _ op) x) <->
+  w' = witness_update ci w op x /\ callee_obligation ci w op x.
+Proof.
+rewrite /gen_witness_update /gen_callee_obligation /=.
+rewrite /sharedcontractprod /= /gen_callee_obligation.
+rewrite !injK_Some injK_None.
+by tauto.
+Qed.
+
+Lemma shared_right_callee_injP (op : G X) :
+  (w' = gen_witness_update
+      (ci -^- cj) w
+      (effect.injT H Fx G _ op) x /\
+    gen_callee_obligation
+      (ci -^- cj) w
+      (effect.injT H Fx G _ op) x) <->
+  w' = witness_update cj w op x /\ callee_obligation cj w op x.
+Proof.
+rewrite /gen_witness_update /gen_callee_obligation /=.
+rewrite /sharedcontractprod /= /gen_callee_obligation.
+rewrite !injK_Some injK_None.
+by tauto.
+Qed.
+End shared_contract_inj_helpers.
